Coq/src/Vf.v
@@ -5,21 +5,88 @@ Require Import EventStructure Consistency.
 Set Implicit Arguments.
 
 Section Vf.
-  Variable A : Type.
-  Variable lab : A -> label.
-  Variable rf : relation A.
-  Variable hb : relation A.
-  Variable sc : relation A.
+Variable A : Type.
+Variable E : A -> Prop.
+Variable lab : A -> label.
+Variable rf : relation A.
+Variable hb : relation A.
+Variable sc : relation A.
 
-  Notation "'W'" := (fun a => is_true (is_w lab a)).
-  Notation "'F'" := (fun a => is_true (is_f lab a)).
-  Notation "'Sc'" := (fun a => is_true (is_sc lab a)).
+Notation "'W'" := (fun a => is_true (is_w lab a)).
+Notation "'F'" := (fun a => is_true (is_f lab a)).
+Notation "'Sc'" := (fun a => is_true (is_sc lab a)).
   
-  Definition vf : relation A := ⦗ W ⦘ ⨾ rf^? ⨾ (hb ⨾ ⦗ F∩₁Sc ⦘)^? ⨾ sc^? ⨾ hb^?.
+Definition Avf : relation A := ⦗ W ⦘ ⨾ rf^? ⨾ (hb ⨾ ⦗ F∩₁Sc ⦘)^? ⨾ sc^? ⨾ hb^? ;; <| E |>.
 End Vf.
 
 Definition Gvf (G : execution) :=
-  vf G.(lab) G.(rf) G.(imm_hb.hb) G.(imm.psc).
+  Avf G.(acts_set) G.(lab) G.(rf) G.(imm_hb.hb) G.(imm.psc).
 
 Definition Svf (m : model) (S : ES.t) :=
-  vf S.(ES.lab) S.(ES.jf) S.(Consistency.hb) (Consistency.psc S m).
+  Avf S.(ES.acts_set) S.(ES.lab) S.(ES.jf) S.(Consistency.hb) (Consistency.psc S m).
+
+Section GvfProperties.
+Variable G : execution.
+Variable WF : Wf G.
+
+Notation "'E'" := G.(acts_set).
+Notation "'psc'" := G.(imm.psc).
+Notation "'hb'" := G.(imm_hb.hb).
+Notation "'rf'" := G.(rf).
+Notation "'lab'" := G.(lab).
+Notation "'vf'" := (Gvf G).
+Notation "'W'" := (fun a => is_true (is_w lab a)).
+Notation "'F'" := (fun a => is_true (is_f lab a)).
+Notation "'Sc'" := (fun a => is_true (is_sc lab a)).
+
+Lemma GvfE : vf ≡ <| E |> ;; vf ;; <| E |>.
+Proof.
+  split; [|basic_solver].
+  unfold Gvf, Avf.
+  rewrite (wf_rfE WF) at 1.
+  rewrite (wf_hbE WF) at 1 2.
+  rewrite (wf_pscE WF) at 1.
+  basic_solver 21.
+Qed.
+
+(* Lemma vf_hb_irr l WF WF_SC CSC COH ACYC_EXT: irreflexive (vf ⨾ hb). *)
+(* Proof. *)
+(*   unfold vf. *)
+(*   arewrite_id ⦗W_ l⦘. *)
+(*   arewrite_id ⦗F ∩₁ Sc⦘. *)
+(*   rels. *)
+
+(*   arewrite (rf^? ⊆ eco^?). *)
+(*   generalize (eco_trans WF); ins; relsf. *)
+(*   rewrite (crE sc). *)
+
+(*   generalize (@hb_trans G); ins; relsf. *)
+
+(*   relsf; repeat (splits; try apply irreflexive_union). *)
+(*   - *)
+(*       by rotate 1; apply COH. *)
+(*   -  *)
+(*     rewrite crE at 1; relsf; repeat (splits; try apply irreflexive_union). *)
+(*     * rotate 1; relsf. *)
+(*       rewrite (wf_scD WF_SC). *)
+(*       rotate 1. *)
+(*       sin_rewrite (f_sc_hb_f_sc_in_sc WF WF_SC ACYC_EXT). *)
+(*       destruct WF_SC; relsf. *)
+(*     *  *)
+(*       rewrite (wf_scD WF_SC), !seqA. *)
+(*       rewrite crE; relsf; apply irreflexive_union; splits; *)
+(*         [rewrite (dom_r (wf_ecoD WF)); type_solver|]. *)
+(*       revert CSC; unfold coh_sc; basic_solver 21. *)
+(* Qed. *)
+
+(* Lemma Gvf_hb_sc_hb_irr WF WF_SC CSC COH ACYC_EXT l: *)
+(*   irreflexive (vf ⨾ hb ⨾ (sc ⨾ hb)^?). *)
+(* Proof. *)
+(* case_refl _. *)
+(* apply (vf_hb_irr WF WF_SC CSC COH ACYC_EXT). *)
+(* arewrite (vf ⨾ hb ⨾ sc ⊆ vf). *)
+(* generalize (@vf_hb_sc_hb l WF WF_SC ACYC_EXT); basic_solver 21. *)
+(* apply (vf_hb_irr WF WF_SC CSC COH ACYC_EXT). *)
+(* Qed. *)
+
+End GvfProperties.
