Coq/src/CertRf.v
@@ -1,0 +1,244 @@
+Require Import Program.Basics.
+From hahn Require Import Hahn.
+From imm Require Import Events Execution TraversalConfig
+     imm imm_hb CertExecution2.
+Require Import Vf.
+
+Section CertRf.
+Variable G  : execution.
+Variable sc : relation actid.
+Variable TC : trav_config.
+Variable thread : thread_id.
+
+Notation "'C'"  := (covered TC).
+Notation "'I'"  := (issued TC).
+
+Notation "'D'" := (D G TC thread).
+
+Notation "'E'" := G.(acts_set).
+Notation "'lab'" := (G.(lab)).
+Notation "'rmw'" := G.(rmw).
+
+Notation "'Tid_' t" := (fun x => tid x = t) (at level 1).
+Notation "'NTid_' t" := (fun x => tid x <> t) (at level 1).
+
+Notation "'R'" := (fun a => is_true (is_r lab a)).
+Notation "'W'" := (fun a => is_true (is_w lab a)).
+
+Notation "'sb'" := (G.(sb)).
+Notation "'hb'" := (G.(imm_hb.hb)).
+Notation "'psc'" := (G.(imm.psc)).
+Notation "'rf'" := (G.(rf)).
+Notation "'co'" := (G.(co)).
+Notation "'vf'" := (G.(Gvf)).
+Notation "'loc'" := (loc lab).
+
+Notation "'Loc_' l" := (fun x => loc x = Some l) (at level 1).
+Notation "'W_' l" := (W ∩₁ Loc_ l) (at level 1).
+Notation "'R_' l" := (R ∩₁ Loc_ l) (at level 1).
+
+Definition cert_rf :=
+  vf ∩ same_loc lab ⨾ ⦗ (E \₁ D) ∩₁ R ⦘ \ co ⨾ vf.
+Definition cert_rfi := ⦗  Tid_ thread ⦘ ⨾ cert_rf ⨾ ⦗ Tid_ thread ⦘.
+Definition cert_rfe := ⦗ NTid_ thread ⦘ ⨾ cert_rf ⨾ ⦗ Tid_ thread ⦘.
+
+Section Properties.
+Variable WF  : Wf G.
+Variable COH : imm_consistent G.
+  
+Lemma cert_rfE : cert_rf ≡ ⦗E⦘ ⨾ cert_rf ⨾ ⦗E \₁ D⦘.
+Proof.
+  apply dom_helper_3.
+  unfold cert_rf.
+  rewrite (GvfE WF).
+  basic_solver 21.
+Qed.
+
+Lemma cert_rfD : cert_rf ≡ ⦗W⦘ ⨾ cert_rf ⨾ ⦗R⦘.
+Proof.
+  apply dom_helper_3.
+  unfold cert_rf.
+  unfold Gvf, Avf.
+  basic_solver.
+Qed.
+
+Lemma cert_rfl : cert_rf ⊆ same_loc lab.
+Proof. unfold cert_rf. basic_solver. Qed.
+
+Lemma cert_rff : functional cert_rf⁻¹.
+Proof.
+  rewrite cert_rfD, cert_rfE.
+  red. intros x y z AA BB.
+  assert (exists l, loc y = Some l) as HH.
+  { generalize (is_w_loc lab). unfolder in *.
+    basic_solver 12. }
+  desc.
+
+  assert (loc z = Some l) as GG.
+  { hahn_rewrite cert_rfl in AA.
+    hahn_rewrite cert_rfl in BB.
+    unfold same_loc in *.
+    unfolder in *.
+    desf. congruence. }
+
+  unfolder in *.
+  destruct (classic (y=z)) as [|X]; eauto; desf.
+  exfalso.
+  eapply wf_co_total in X; try basic_solver 22.
+  2: { unfolder. splits; eauto. congruence. }
+  unfold cert_rf in *. desf; unfolder in *; basic_solver 40.
+Qed.
+
+Lemma cert_rf_comp : forall b (IN: ((E \₁ D) ∩₁ R) b), exists a, cert_rf a b.
+Proof.
+  ins; unfolder in *; desf.
+  assert (exists l, loc b = Some l); desc.
+  { by generalize (is_r_loc lab); unfolder in *; basic_solver 12. }
+  assert (E (InitEvent l)).
+  { by apply WF; eauto. }
+  assert (lab (InitEvent l) = Astore Xpln Opln l 0).
+  { by apply WF. }
+  assert (loc (InitEvent l) = Some l).
+  { by unfold Events.loc; rewrite (wf_init_lab WF). }
+  assert (W_ l (InitEvent l)).
+  { by unfolder; unfold is_w, Events.loc; desf; eauto. }
+  assert (sb (InitEvent l) b).
+  { by apply init_ninit_sb; eauto; eapply read_or_fence_is_not_init; eauto. }
+  assert (vf (InitEvent l) b).
+  { exists (InitEvent l); splits.
+    { red. splits; desf. by apply WF.(init_w). }
+    unfold eqv_rel; eauto.
+    hahn_rewrite <- sb_in_hb.
+    basic_solver 21. }
+
+  forward (eapply last_exists with (s:=co ⨾ ⦗fun x => vf x b⦘) 
+                                   (dom:= filterP (W_ l) G.(acts)) (a:=(InitEvent l))).
+  { eapply acyclic_mon.
+    apply trans_irr_acyclic; [apply co_irr| apply co_trans]; eauto.
+    basic_solver. }
+  { ins.
+    assert (A: (co ⨾ ⦗fun x : actid => vf x b⦘)^? (InitEvent l) c).
+    { apply rt_of_trans; try done.
+      apply transitiveI; unfolder; ins; desf; splits; eauto.
+      eapply co_trans; eauto. }
+    unfolder in A; desf.
+    { by apply in_filterP_iff; split; auto. }
+    apply in_filterP_iff.
+    hahn_rewrite WF.(wf_coE) in A.
+    hahn_rewrite WF.(wf_coD) in A.
+    hahn_rewrite WF.(wf_col) in A.
+    unfold same_loc in *; unfolder in *; desf; splits; eauto; congruence. }
+  ins; desf.
+  assert (A: (co ⨾ ⦗fun x : actid => vf x b⦘)^? (InitEvent l) b0).
+  { apply rt_of_trans; try done.
+    apply transitiveI; unfolder; ins; desf; splits; eauto.
+    eapply co_trans; eauto. }
+  assert (loc b0 = Some l).
+  { unfolder in A; desf.
+    hahn_rewrite WF.(wf_col) in A.
+    unfold same_loc in *; desf; unfolder in *; congruence. }
+  exists b0; red; split.
+  { unfold Gvf, Avf, same_loc.
+    unfolder in A; desf; unfolder; ins; desf; splits; try basic_solver 21; congruence. }
+  unfold max_elt in *.
+  unfolder in *; ins; desf; intro; desf; basic_solver 11.
+Qed.
+
+Lemma cert_rf_mod: (E \₁ D) ∩₁ R ≡₁ codom_rel cert_rf.
+Proof.
+  split.
+  unfolder; ins; desf.
+  apply cert_rf_comp; basic_solver.
+  unfold cert_rf; basic_solver.
+Qed.
+
+Lemma cert_rf_in_vf: cert_rf ⊆ vf.
+Proof. unfold cert_rf; basic_solver. Qed.
+
+(* Lemma cert_rf_hb: irreflexive (cert_rf ⨾ hb ⨾ (psc ⨾ hb)^?). *)
+(* Proof. *)
+(*   rewrite cert_rf_in_vf. *)
+(*   apply furr_hb_sc_hb_irr; done. *)
+(* Qed. *)
+
+(* Lemma non_I_cert_rf: ⦗E \₁ I⦘ ⨾ cert_rf ⊆ Gsb. *)
+(* Proof. *)
+(* assert (cert_rf_hb: irreflexive (cert_rf ⨾ Ghb ⨾ (sc ⨾ Ghb)^?)). *)
+(* by apply cert_rf_hb. (* Coq bug ?! *) *)
+
+(* rewrite (cert_rfD). *)
+(* arewrite (⦗E \₁ I⦘ ⨾ ⦗W⦘ ⊆ ⦗E \₁ I⦘ ⨾ ⦗Tid_ thread⦘ ⨾ ⦗W⦘). *)
+(* by revert IT_new_co; unfolder; firstorder. *)
+(* rewrite (cert_rfE). *)
+(* arewrite (E \₁ D ⊆₁ E ∩₁ Tid_ thread). *)
+(* by unfold D; unfolder; ins; desf; tauto. *)
+(* unfolder; ins; desf. *)
+(* eapply (@same_thread G) in H3; desf. *)
+(* destruct H3; [subst x; type_solver|]. *)
+(* 2: by intro K; apply (init_w WF) in K; type_solver. *)
+(* exfalso; generalize cert_rf_hb. *)
+(* generalize (@sb_in_hb G); basic_solver 12. *)
+(* Qed. *)
+
+(* Lemma cert_rfe_Acq : (cert_rf \ Gsb) ⨾ ⦗R∩₁Acq⦘ ⊆ ∅₂. *)
+(* Proof. *)
+(* rewrite cert_rfE. *)
+(* arewrite (⦗E⦘ ⊆ ⦗E \₁ I⦘ ∪ ⦗E ∩₁ I⦘). *)
+(* unfolder; ins; desf; tauto. *)
+(* relsf. *)
+(* rewrite minus_union_l. *)
+(* relsf; unionL. *)
+(* sin_rewrite non_I_cert_rf. *)
+(* basic_solver. *)
+(* rewrite cert_rfD. *)
+(* arewrite (cert_rf ⊆ cert_rf ∩ Gsame_loc). *)
+(* generalize (cert_rfl); basic_solver. *)
+
+(* unfolder; ins; desf. *)
+
+(* assert (Lx:exists l, Gloc x = Some l); desc. *)
+(* by apply is_w_loc. *)
+
+(* assert (Ly:Gloc y = Some l). *)
+(* unfold same_loc in *; congruence. *)
+
+(* forward (apply COMP_ACQ). *)
+(* by basic_solver. *)
+
+(* ins; desc. *)
+
+(* apply rfi_union_rfe in H10; unfolder in H10; desf; cycle 1. *)
+(* by generalize R_Acq_codom_rfe; basic_solver 12. *)
+
+(* ie_unfolder; unfolder in H10; desf. *)
+
+(* hahn_rewrite (wf_rfD WF) in H10. *)
+(* hahn_rewrite (wf_rfE WF) in H10. *)
+
+(* unfolder in H10; desf. *)
+
+(* assert (Lz:Gloc z = Some l). *)
+(* by apply (wf_rfl WF) in H14; unfold same_loc in *; congruence. *)
+
+(* forward (apply ((wf_co_total WF) (Some l) z)). *)
+(* basic_solver. *)
+(* instantiate (1 := x). *)
+(* basic_solver. *)
+
+(* intro; desf. *)
+
+(* intro; desf. *)
+
+(* - *)
+(* eapply eco_furr_irr; try edone. *)
+(* eexists; splits; [|eby apply cert_rf_in_furr]. *)
+(* unfold eco, fr. *)
+(* basic_solver 12. *)
+(* - eapply H3. *)
+(* exists z; split; [| apply furr_alt; basic_solver 12]. *)
+(* apply I_co_in_cert_co; basic_solver. *)
+(* Qed. *)
+
+End Properties.
+
+End CertRf.
